<?xml version='1.0' encoding='utf-8'?>

<section xml:id="S_bicond">
  <title>Proofs of Biconditional Statements</title>
  <idx><h>Pythagorean Theorem</h></idx>
  <p>
    One of the logical equivalencies in <xref ref="thm-log-equiv"/> is the following one for biconditional statements.
    <me>
      \left( P \leftrightarrow Q \right) \equiv \left( P \to Q \right) \wedge \left( Q \to P \right)
    </me>
    This logical equivalency suggests one method for proving a biconditional statement written in the form <q><m>P</m> if and only if <m>Q</m>.</q> This method is to construct separate proofs of the two conditional statements <m>P \to Q</m> and <m>Q \to P</m>.
  </p>
  <p>
    We will illustrate this with a proposition about right triangles.
  </p>
  <p>
    Recall that the <term>Pythagorean Theorem</term> for right triangles states that if <m>a</m> and <m>b</m> are the lengths of the legs of a right triangle and <m>c</m> is the length of the hypotenuse, then <m>a^2 + b^2 = c^2</m> . We also know that the area of any triangle is one-half the base times the altitude. So for the right triangle we have described, the area is <m>A = \frac{1}{2} ab</m>.
  </p>

  <proposition xml:id="prop-triangle">
    <statement>
      <p>
        Suppose that <m>a</m> and <m>b</m> are the lengths of the legs of a right triangle and <m>c</m> is the length of the hypotenuse. This right triangle is an isosceles triangle if and only if the area of the right triangle is <m>\frac{1}{4} c^2</m>.
      </p>
    </statement>
    <proof>
      <p>
        We assume that we have a right triangle where <m>a</m> and <m>b</m> are the lengths of the legs of a right triangle and <m>c</m> is the length of the hypotenuse. We will prove that this right triangle is an isosceles triangle if and only if the area of the right triangle is <m>\frac{1}{4} c^2</m> by proving the two conditional statements associated with this biconditional statement.
      </p>
      <p>
        We first prove that if this right triangle is an isosceles triangle, then the area of the right triangle is <m>\frac{1}{4} c^2</m>. So we assume the right triangle is an isosceles triangle. This means that <m>a = b</m>, and consequently, <m>A = \frac{1}{2} a^2</m>. Using the Pythagorean Theorem, we see that
        <me>
          c^2 = a^2 + a^2 = 2a^2
        </me>.
        Hence, <m>a^2 = \frac{1}{2} c^2</m>, and we obtain <m>A = \frac{1}{2} a^2 = \frac{1}{4} c^2</m>. This proves that if this right triangle is an isosceles triangle, then the area of the right triangle is <m>\frac{1}{4} c^2</m>.
      </p>
      <p>
        We now prove the converse of the first conditional statement. So we assume the area of this isosceles triangle is <m>A = \frac{1}{4} c^2</m> , and will prove that <m>a = b</m>. Since the area is also <m>\frac{1}{2} ab</m>, we see that
        <md>
          <mrow>\frac{1}{4} c^2 \amp = \frac{1}{2}ab</mrow>
          <mrow>c^2 \amp = 2ab</mrow>
        </md>
        We now use the Pythagorean Theorem to conclude that <m>a^2 + b^2 = 2ab</m>. So the last equation can be rewritten as follows:
        <md>
          <mrow>a^2 - 2ab + b^2 \amp = 0</mrow>
          <mrow>(a - b)^2 \amp = 0</mrow>
        </md>.
        The last equation implies that <m>a = b</m> and hence the right triangle is an isosceles triangle. This proves that if the area of this right triangle is <m>A = \frac{1}{4} c^2</m>, then the right triangle is an isosceles triangle.
      </p>
      <p>
        Since we have proven both conditional statements, we have proven that this right triangle is an isosceles triangle if and only if the area of the right triangle is <m>\frac{1}{4} c^2</m>.
      </p>
    </proof>
  </proposition>
  
</section>