<?xml version='1.0' encoding='utf-8'?>

<section xml:id="S_dne">
  <title>Proving that Something Does Not Exist</title>

  <p>
    In mathematics, we sometimes need to prove that something does not exist or that something is not possible. Instead of trying to construct a direct proof, it is sometimes easier to use a proof by contradiction so that we can assume that the something exists.
  </p>
  <p>
    We will illustrate this by proving the following proposition. Notice that the conclusion of the proposition involves trying to prove that an integer with a certain property does not exist. If we use a proof by contradiction, we can assume that such an integer <m>z</m> exists. This gives us more with which to work.
  </p>

  <proposition xml:id="prop-dne-odd">
    <statement>
      <p>
        For all integers <m>x</m> and <m>y</m>, if <m>x</m> and <m>y</m> are odd integers, then there does not exist an integer <m>z</m> such that <m>x^2 + y^2 = z^2</m>.
      </p>
    </statement>
    <proof>
      <p>
        We will use a proof by contradiction. So we assume that the proposition is false or that there exist integers <m>x</m> and <m>y</m> such that <m>x</m> and <m>y</m> are odd and there exists an integer <m>z</m> such that <m>x^2 + y^2 = z^2</m>. Since <m>x</m> and <m>y</m> are odd, there exist integers <m>m</m> and <m>n</m> such that <m>x = 2m + 1</m> and <m>y = 2n + 1</m>. So we get
        <mdn>
          <mrow number='no'>x^2 + y^2 \amp = (2m + 1)^2 + (2n + 1)^2</mrow>
          <mrow number='no'> \amp = 4m^2 + 4m + 1 + 4n^2 + 4n + 1</mrow>
          <mrow xml:id="dne-odd-mn"> \amp = 2 ( 2m^2 + 2m + 2n^2 + 2n + 1 )</mrow>
        </mdn>
        Since the integers are closed under addition and multiplication, we see that <m>2 ( 2m^2 + 2m + 2n^2 + 2n + 1 )</m> is an integer, and so the last equation shows that <m>x^2 + y^2</m> is an even integer. Hence, <m>z^2</m> is even since <m>z^2 = x^2 + y^2</m> . So using the result in <xref ref="prop-even-squared" />, we can conclude that <m>z</m> is even and that there exists an integer <m>k</m> such that <m>z = 2k</m>. Now, using equation <xref ref="dne-odd-mn"/> above, we see that
        <md>
          <mrow>z^2 \amp = 2 (2m^2 + 2m + 2n^2 + 2n + 1)</mrow>
          <mrow>2k^2 \amp = 2 (2m^2 + 2m + 2n^2 + 2n + 1)</mrow>
          <mrow>4k^2 \amp = 2 (2m^2 + 2m + 2n^2 + 2n + 1)</mrow>
        </md>
        Dividing both sides of the last equation by 2, we obtain
        <md>
          <mrow>4k^2 \amp = 2 (2m^2 + 2m + 2n^2 + 2n + 1)</mrow>
          <mrow>2k^2 \amp = 2 (m^2 + m + n^2 + n) + 1</mrow>
        </md>
      </p>
      <p>
        However, the left side of the last equation is an even integer and the right side is an odd integer. This is a contradiction, and so the proposition cannot be false. Hence, we have proved that for all integers <m>x</m> and <m>y</m>, if <m>x</m> and <m>y</m> are odd integers, then there does not exist an integer <m>z</m> such that <m>x^2 + y^2 = z^2</m>. 
      </p>
    </proof>
  </proposition>
  
</section>