<?xml version='1.0' encoding='utf-8'?>

<section xml:id="S_induct_exer">
  <title>Practice Problems for <xref ref="C_induction"/></title>
  
  <exercises>
    <title></title>
    
    <exercise>
      <task xml:id="exer-natural-nums">
        <statement>
          <p>
            Calculate <m>1 + 3 + 5 + \cdots + (2n - 1)</m> for several natural numbers <m>n</m>.
          </p>
        </statement>
      </task>

      <task xml:id="exer-natural-conj">
        <statement>
          <p>
            Based on your work in <xref ref="exer-natural-nums"/>, if <m>n \in N</m>, make a conjecture about the value of the sum <m>1 + 3 + 5 + \cdots + (2n - 1) = \sum_{j = 1}^{n} (2j - 1)</m>.
          </p>
        </statement>
      </task>

      <task>
        <statement>
          <p>
            Use mathematical induction to prove your conjecture in <xref ref="exer-natural-conj"/>.
          </p>
        </statement>
        <solution>
          <proof>
            <p>
              We will use a proof by mathematical induction. For each natural number <m>n</m>, we let <m>P(n)</m> be
              <me>
                1 + 3 + 5 + \cdots + (2n - 1) = n^2
              </me>
              We first prove that <m>P (1)</m> is true. Notice that when <m>n = 1</m>, both the left and right sides of the equation for <m>P (n)</m> are equal to 1. This proves that <m>P(1)</m> is true.
            </p>
            <p>
              For the inductive step, we prove that for each <m>k \in \N</m>, if <m>P (k)</m> is true, then <m>P (k + 1)</m> is true. So let <m>k</m> be a natural number and assume that <m>P (k)</m> is true. That is, assume that
              <men xml:id="eqn-induct-sol1">
                1 + 3 + 5 + \cdots + (2k - 1) = k^2
              </men>.
              The goal now is to prove that <m>P (k + 1)</m> is true. That is, it must be proved that
              <mdn>
                <mrow number='no'>1 + 3 + 5 + \cdots + (2k - 1) + (2(k + 1) - 1) \amp = (k + 1)^2</mrow>
                <mrow xml:id="eqn-induct-sol2">1 + 3 + 5 + \cdots + (2k - 1) + (2k + 1) \amp = (k + 1)^2</mrow>
              </mdn>
              To do this, we add <m>(2k + 1)</m> to both sides of equation <xref ref="eqn-induct-sol1"/>, which gives
              <md>
                <mrow>1 + 3 + 5 + \cdots + (2k - 1) + (2k + 1) \amp = k^2 + k + 1</mrow>
                <mrow> \amp = (k + 1)^2</mrow>
              </md>
              Comparing this result to equation <xref ref="eqn-induct-sol2"/>, we see that if <m>P (k)</m> is true, then <m>P (k + 1)</m> is true. Hence, the inductive step has been established, and by the Principle of Mathematical Induction, we have proved that for each natural number <m>n</m>, <m>1 + 3 + 5 + \cdots + (2n - 1) = n^2</m>.
            </p>
          </proof>
        </solution>
      </task>
    </exercise>

    <exercise>
      <statement>
        <p>
          Prove the following:
          <blockquote>
            Proposition. For each natural number <m>n</m>, 3 divides <m>\modulo{4^n}{1}{3}</m>.
          </blockquote>
        </p>
      </statement>
      <solution>
        <proof>
          <p>
            We will use a proof by mathematical induction. For each natural number <m>n</m>, we let <m>P (n)</m> be
            <me>
              \modulo{4^n}{1}{3}
            </me>
            We first prove that <m>P (1)</m> is true. Notice that when <m>n = 1</m>, <m>4^n = 4^1 = 4</m> and <m>\modulo{4}{1}{3}</m>. This proves that <m>P (1)</m> is true.
          </p>
          <p>
            For the inductive step, we prove that for each <m>k \in \N</m>, if <m>P (k)</m> is true, then <m>P (k + 1)</m> is true. So let <m>k</m> be a natural number and assume that <m>P (k)</m> is true. That is, assume that
            <men xml:id="eqn-induct-sol3">
              \modulo{4^k}{1}{3}
            </men>
            The goal now is to prove that <m>P (k + 1)</m> is true. That is, it must be proved that
            <men xml:id="eqn-induct-sol4">
              \modulo{4^{k+1}}{1}{3}
            </men>
            Since we have to assume that <m>\modulo{4^k}{1}{3}</m>, we conclude that 3 divides <m>\left( 4^k + 1 \right)</m> and so there exists and integer <m>m</m> such that
            <me>
              4^k - 1 = 3m
            </me>.
            Multiplying both sides of this equation by 4, we obtain
            <md>
              <mrow>4 \left( 4^k + 1 \right) \amp = 4(3m)</mrow>
              <mrow>4^{k + 1} - 4 \amp = 12m</mrow>
              <mrow>4^{k + 1} - 3 - 1 \amp = 12m</mrow>
              <mrow>4^{k + 1} - 1 \amp = 3 + 12m</mrow>
              <mrow>4^{k + 1} -  \amp 3( 1 + 4m)</mrow>
            </md>
             So we have proved that if <m>P (k)</m> is true, then <m>P (k + 1)</m> is true. Hence, the inductive step has been established, and by the Principle of Mathematical Induction, we have proved that for each natural number <m>n</m>, <m>\modulo{4^n}{1}{3}</m>.
          </p>
        </proof>
      </solution>
    </exercise>

    <exercise>
      <statement>
        <p>
          For which natural numbers <m>n</m> is <m>3^n</m> greater than <m>5 + 2^n</m>? State a proposition (with an appropriate quantifier) and prove it.
        </p>
      </statement>
      <solution>
        <p>
          <blockquote>
            Proposition. For each natural number <m>n</m> with <m>n \geq 3</m>, <m>3^n \gt 5 + 2^n</m>.
          </blockquote>
        </p>
        <proof>
          <p>
            We will use a proof by mathematical induction. For each natural number <m>n</m>, we let <m>P (n)</m> be
            <me>
              3^n \gt 5 + 2^n
            </me>
            We first prove that <m>P (3)</m> is true. Notice that when <m>n = 3</m>, <m>3^n = 27</m> and <m>5 + 2^n = 13</m>. Since <m>27 \gt 13</m>, this proves that <m>P (1)</m> is true.
          </p>
          <p>
            For the inductive step, we prove that for each <m>k \in \N</m> with <m>k \geq 3</m>, if <m>P (k)</m> is true, then <m>P (k + 1)</m> is true. So let <m>k</m> be a natural number with <m>k \geq 3</m> and assume that <m>P (k)</m> is true. That is, assume that
            <men xml:id="eqn-induct-sol5">
              3^k \gt 5 + 2^k
            </men>
            The goal now is to prove that <m>P (k + 1)</m> is true. That is, it must be proved that
            <men xml:id="eqn-induct-sol6">
              3^{k+1} \gt 5 + 2^{k+1}
            </men>
            So we multiply both sides of inequality <xref ref="eqn-induct-sol5"/> to obtain
            <mdn>
              <mrow number='no'>3 \cdot 3^k \amp \gt 3(5 + 2^k)</mrow>
              <mrow xml:id="eqn-induct-sol7">3^{k + 1} \amp \gt 15 + 3 \cdot 2^k</mrow>
            </mdn>
            Since <m>3 \gt 2</m>, <m>3 \cdot 2^k > 2 \cdot 2^k</m> or <m>3 \cdot 2^k > 2^{k+1}</m>. In addition, <m>15 \gt 5</m> and so we can co
          </p>
          <p>
            So we have proved that if <m>P (k)</m> is true, then <m>P (k + 1)</m> is true. Hence, the inductive step has been established, and by the Principle of Mathematical Induction, we have proved that for each natural number <m>n</m>, <m>\modulo{4^n}{1}{3}</m>.
          </p>
        </proof>
      </solution>
    </exercise>

    <exercise>
    <idx><h>Fibonacci numbers</h></idx>
      <introduction>
        <p>
          The <term>Fibonacci numbers</term> are a sequence of natural numbers <m>f_1, f_2, f_3, \ldots, f_n, \ldots</m> defined recursively as follows:
          <ul>
            <li>
              <p>
                <m>f_1 = 1</m> and <m>f_2 = 1</m>, and
              </p>
            </li>
            <li>
              <p>
                For each natural number <m>n</m>, <m>f_{n + 2} = f_{n + 1} + f_n</m>.
              </p>
            </li>
          </ul>
          In words, the recursion formula states that for any natural number <m>n</m> with <m>n =\geq 3</m>, the <m>n^{th}</m> Fibonacci number is the sum of the two previous Fibonacci numbers. So we see that
          <md>
            <mrow>f_3 \amp = f_2 + f_1 = 1 + 1 = 2</mrow>
            <mrow>f_4 \amp = f_3 + f_2 = 2 + 1 = 3 \text{, and }</mrow>
            <mrow>f_5 \amp = f_4 + f_3 = 3 + 2 = 5</mrow>
          </md>
        </p>
      </introduction>

      <task>
        <statement>
          <p>
            Calculate <m>f_6</m> through <m>f_{20}</m>.
          </p>
        </statement>
        <solution>
          <p>
            <md>
              <mrow>f(5) \amp = 5 \amp f_9 \amp = 34 \amp f_{13} \amp = 233 \amp f(17) \amp = 1597</mrow>
              <mrow>f(6) \amp = 8 \amp f_{10} \amp = 55 \amp f_{14} \amp = 377 \amp f(18) \amp = 2584</mrow>
              <mrow>f(7) \amp = 13 \amp f_{11} \amp = 89 \amp f_{15} \amp = 610 \amp f(19) \amp = 4181</mrow>
              <mrow>f(8) \amp = 21 \amp f_{12} \amp = 144 \amp f_{16} \amp = 987 \amp f(20) \amp = 6765</mrow>
            </md>
          </p>
        </solution>
      </task>

      <task>
        <statement>
          <p>
            Is every third Fibonacci number even? That is it true that for each natural number <m>n</m>, <m>f_{3n}</m> is even? Justify your conclusion.
          </p>
        </statement>
        <solution>
          <proof>
            <p>
              We will use a proof by induction. For each natural number <m>n</m>, we let <m>P (n)</m> be,
              <blockquote>
                <m>f_{3n}</m> is an even natural number.
              </blockquote>
              Since <m>f_3 = 2</m>, we see that <m>P (1)</m> is true and this proves the basis step.
            </p>
            <p>
              For the inductive step, we let <m>k</m> be a natural number and assume that <m>P (k)</m> is true. That is, assume that <m>f_{3k}</m> is an even natural number. This means that there exists an integer <m>m</m> such that
              <men xml:id="eqn-induct-sol8">
                f_{3k} = 2m
              </men>.
              We need to prove that <m>P (k + 1)</m> is true or that <m>f_{3(k+1)}</m> is even. Notice that <m>3(k + 1) = 3k + 3</m> and, hence, <m>f_{3(k+1)} = f_{3k+3}</m>. We can now use the recursion formula for the Fibonacci numbers to conclude that
              <me>
                f_{3k+3} = f_{3k+2} + f_{3k+1}
              </me>.
              Using the recursion formula again, we get <m>f_{3k+2} = f_{3k+1} + f_{3k}</m>. Putting this all together, we see that
              <mdn>
                <mrow number='no'>f_{3(k+1)} \amp = f_{3k+3}</mrow>
                <mrow number='no'> \amp = f_{3k+2} + f_{3k+1}</mrow>
                <mrow number='no'> \amp = (f_{3k+1} + f_{3k}) + f_{3k+1}</mrow>
                <mrow xml:id="eqn-induct-sol9"> \amp = 2 f_{3k+1} + f_{3k}</mrow>
              </mdn>
              We now substitute the expression for <m>f_{3k}</m> in equation <xref ref="eqn-induct-sol8"/> into equation <xref ref="eqn-induct-sol9"/>. This gives
              <md>
                <mrow>f_{3(k+1)} \amp = 2 f_{3k+1} + 2m</mrow>
                <mrow>f_{3(k+1)} \amp = 2 (f_{3k+1} + m)</mrow>
              </md>
              This preceding equation shows that <m>f_{3(k+1)}</m> is even. Hence it has been proved that if <m>P (k)</m> is true, then <m>P (k + 1)</m> is true and the inductive step has been established. By the Principle of Mathematical Induction, this proves that for each natural number <m>n</m>, the Fibonacci number <m>f_{3n}</m> is an even natural number. 
            </p>
          </proof>
        </solution>
      </task>

      <task>
        <statement>
          <p>
            Is it true that for each natural number <m>n</m> with <m>n \geq 2</m>, <m>f_1 + f_3 + \cdots + f_{2n-1} = f_{n + 1} - 1</m>? Justify your conclusion.
          </p>
        </statement>
        <solution>
          <proof>
            <p>
              Let P(n) be <q><m>f_1 + f_2 + \cdots + f_{n-1} = f_{n + 1} -1</m>.</q> Since <m>f_1 = f_3 - 1</m>, <m>P(2)</m> is true, and this proves the basis step.
            </p>
            <p>
              For the inductive step, we let <m>k</m> be a natural number with <m>k \geq 2</m> and assume that <m>P (k)</m> is true and will prove that <m>P (k + 1)</m> is true. That is, we assume that
              <men xml:id="eqn-induct-sol10">
                f_1 + f_2 + \cdots + f_{k-1} = f_{k + 1} -1
              </men>,
              and will prove that
              <men xml:id="eqn-induct-sol11">
                f_1 + f_2 + \cdots + f_{k-1} + f_k = f_{(k + 1) + 1} - 1 = f_{k+2} - 1
              </men>.
              By adding <m>f_k</m> to both sides of equation <xref ref="eqn-induct-sol10"/>, we see that
              <md>
                <mrow>(f_1 + f_2 + \cdots + f_{k-1}) + f_k \amp = (f_{k + 1} - 1) + f_k</mrow>
                <mrow> \amp = (f_{k + 1} + f_k) - 1</mrow>
                <mrow> \amp = f_{k + 2} - 1</mrow>
              </md>.
              Comparing this to equation <xref ref="eqn-induct-sol11"/>, we see that we have proved that if <m>P (k)</m> is true, then <m>P (k + 1)</m> is true and the inductive step has been established. So by the Principle of Mathematical Induction, this proves that for each natural number n with <m>n \geq 2 </m>, <m>f_1 + f_3 + \cdots + f_{2n-1} = f_{n + 1} - 1</m>
            </p>
          </proof>
        </solution>
      </task>
    </exercise>
    
    <exercise>
      <statement>
        <p>
          Prove the following proposition using mathematical induction.
          <blockquote>
            For each <m>n \in \N</m> with <m>n \geq 8</m>, there exist nonnegative integers <m>x</m> and <m>y</m> such that <m>n = 3x + 5y</m>.
          </blockquote>
        </p>
        <p>
          Suggestion: Use the Second Principle of Induction and have the basis step be a proof that <m>P(8)</m>, <m>P(9)</m>, and <m>P (10)</m> are true using an appropriate open sentence for <m>P(n)</m>.
        </p>
      </statement>
      <solution>
        <proof>
          <p>
            Proof. We will use a proof by mathematical induction. We let <m>P(n)</m> be, <q>there exist nonnegative integers <m>x</m> and <m>y</m> such that <m>n = 3x + 5y</m>.</q>
          </p>
          <p>
            Basis Step: For the basis step, we will show that <m>P (8)</m>, <m>P (9)</m>, and <m>P (10)</m> are true. We see that
            <ul>
              <li>
                <p>
                  <m>P(8)</m> is true since <m>3 \cdot 1 + 5 \cdot 1 = 8</m>.
                </p>
              </li>
              <li>
                <p>
                  <m>P (9)</m> is true since <m>3 \cdot 3 + 5 \cdot 0 = 9</m>
                </p>
              </li>
              <li>
                <p>
                  <m>P (10)</m> is true since <m>3 \cdot 0 + 5 \cdot 2 = 10</m>.
                </p>
              </li>
            </ul>
          </p>
          <p>
            Inductive Step: Let <m>k \in \N</m> with <m>k \geq 10</m>. Assume that <m>P (8)</m>, <m>P (9)</m>, <ellipsis/>, <m>P (k)</m> are true. Now, notice that
            <me>
              k + 1 = 3 + (k - 2)
            </me>
            Since <m>k \geq 10</m>, we can conclude that <m>k - 2 \geq 8</m> and hence <m>P (k-2)</m> is true. Therefore, there exist non-negative integers <m>u</m> and <m>v</m> such that <m>k - 2 = (3u + 5v)</m>. Using this equation, we see that
            <md>
              <mrow>k + 1 \amp = 3 + (3u + 5v)</mrow>
              <mrow> \amp = 3 ( 1 + u) + 5v</mrow>
            </md>.
            Hence, we can conclude that <m>P (k + 1)</m> is true. This proves that if <m>P (8)</m>, <m>P (9)</m>, <ellipsis/> , <m>P(k)</m> are true, then <m>P (k)</m> is true. Hence, by the Second Principle of Mathematical Induction, for all natural numbers <m>P (k + 1)</m> with <m>n \geq 8</m>, there exist nonnegative integers <m>x</m> and <m>y</m> such that <m>n = 3x + 5y</m>.
          </p>
        </proof>
      </solution>
    </exercise>
    
  </exercises>

</section>